vale/code/arch/x64/X64.Vale.Decls.fsti
@@ -41,11 +41,22 @@ type tainted_operand:eqtype =
 | TMem: m:maddr -> t:taint -> tainted_operand
 
 [@va_qattr]
+type tainted_operand128:eqtype =
+| TReg128: x:xmm -> tainted_operand128
+| TMem128: m:maddr -> t:taint -> tainted_operand128
+
+[@va_qattr]
 unfold let t_op_to_op (t:tainted_operand) : operand =
   match t with
   | TConst n -> OConst n
   | TReg r -> OReg r
   | TMem m _ -> OMem m
+
+[@va_qattr]
+unfold let t_op_to_op128 (t:tainted_operand128) : mov128_op =
+  match t with
+  | TReg128 r -> Mov128Xmm r
+  | TMem128 m _ -> Mov128Mem m
 
 let get_taint (t:tainted_operand) : taint =
   match t with
@@ -78,8 +89,8 @@ unfold let va_codes = list va_code
 let va_tl (cs:va_codes) : Ghost va_codes (requires Cons? cs) (ensures fun tl -> tl == Cons?.tl cs) = Cons?.tl cs
 unfold let va_state = state
 val va_fuel : Type0
-unfold let va_operand = o:tainted_operand
-unfold let va_operand_opr64 = o:va_operand
+unfold let va_operand = tainted_operand
+unfold let va_operand_opr64 = va_operand
 let va_reg_operand = o:va_operand{OReg? (t_op_to_op o)}
 let va_operand_reg_opr64 = o:va_operand{OReg? (t_op_to_op o)}
 unfold let va_dst_operand = o:va_operand
@@ -89,6 +100,8 @@ unfold let va_operand_shift_amt64 = o:va_operand
 unfold let va_cmp = o:va_operand{not (TMem? o)}
 unfold let va_register = reg
 unfold let va_operand_xmm = xmm
+unfold let va_operand128 = tainted_operand128
+unfold let va_operand_opr128 = va_operand128
 
 [@va_qattr] unfold let va_expand_state (s:state) : state = state_eta s
 
@@ -122,27 +135,42 @@ let valid_maddr (addr:int) (s_mem:M.mem) (s_memTaint:M.memtaint) (b:M.buffer64) 
   M.valid_taint_buf64 b s_mem s_memTaint t /\
   addr == M.buffer_addr b s_mem + 8 `op_Multiply` index
 
+let valid_maddr128 (addr:int) (s_mem:M.mem) (s_memTaint:M.memtaint) (b:M.buffer128) (index:int) (t:taint) : prop0 =
+  valid_src_addr s_mem b index /\
+  M.valid_taint_buf128 b s_mem s_memTaint t /\
+  addr == M.buffer_addr b s_mem + 16 `op_Multiply` index
+
 let valid_mem_operand (addr:int) (t:taint) (s_mem:M.mem) (s_memTaint:M.memtaint) : prop0 =
   exists (b:M.buffer64) (index:int).{:pattern (valid_maddr addr s_mem s_memTaint b index t)}
     valid_maddr addr s_mem s_memTaint b index t
+
+let valid_mem_operand128 (addr:int) (t:taint) (s_mem:M.mem) (s_memTaint:M.memtaint) : prop0 =
+  exists (b:M.buffer128) (index:int).{:pattern (valid_maddr128 addr s_mem s_memTaint b index t)}
+    valid_maddr128 addr s_mem s_memTaint b index t
 
 [@va_qattr]
 let valid_operand (t:tainted_operand) (s:state) : prop0 =
   X64.Vale.State.valid_operand (t_op_to_op t) s /\
   (match t with TMem m t -> valid_mem_operand (eval_maddr m s) t s.mem s.memTaint | _ -> True)
 
+[@va_qattr]
+let valid_operand128 (t:tainted_operand128) (s:state) : prop0 =
+  X64.Vale.State.valid_operand128 (t_op_to_op128 t) s /\
+  (match t with TMem128 m t -> valid_mem_operand128 (eval_maddr m s) t s.mem s.memTaint | _ -> True)
+
 (* Constructors *)
 val va_fuel_default : unit -> va_fuel
 [@va_qattr] unfold let va_op_operand_reg (r:reg) : va_operand = TReg r
-[@va_qattr] unfold let va_op_xmm_xmm(x:xmm) : va_operand_xmm = x
+[@va_qattr] unfold let va_op_xmm_xmm (x:xmm) : va_operand_xmm = x
 [@va_qattr] unfold let va_op_opr_reg (r:reg) : va_operand = TReg r
 [@va_qattr] unfold let va_op_opr64_reg (r:reg) : va_operand = TReg r
 [@va_qattr] unfold let va_op_reg64_reg (r:reg) : va_operand = TReg r
+[@va_qattr] unfold let va_op_opr128_xmm (x:xmm) : va_operand128 = TReg128 x
 [@va_qattr] unfold let va_const_operand (n:int) = TConst n
 [@va_qattr] unfold let va_const_opr64 (n:int) = TConst n
 [@va_qattr] unfold let va_const_shift_amt (n:int) : va_shift_amt = TConst n
 [@va_qattr] unfold let va_const_shift_amt64 (n:int) : va_shift_amt = TConst n
-[@va_qattr] unfold let va_op_shift_amt_reg(r:reg) : va_shift_amt = TReg r
+[@va_qattr] unfold let va_op_shift_amt_reg (r:reg) : va_shift_amt = TReg r
 [@va_qattr] unfold let va_op_shift_amt64_reg (r:reg) : va_shift_amt = TReg r
 [@va_qattr] unfold let va_op_cmp_reg (r:reg) : va_cmp = TReg r
 [@va_qattr] unfold let va_const_cmp (n:int) : va_cmp = TConst n
@@ -152,7 +180,7 @@ val va_fuel_default : unit -> va_fuel
 [@va_qattr] unfold let va_coerce_dst_operand_to_reg_operand (o:va_dst_operand{OReg? (t_op_to_op o)}) : va_reg_operand = o
 [@va_qattr] unfold let va_coerce_reg_opr64_to_dst_opr64 (o:va_operand_reg_opr64) : va_operand_dst_opr64 = o
 [@va_qattr] unfold let va_coerce_reg_opr64_to_opr64 (o:va_operand_reg_opr64) : va_operand_opr64 = o
-[@va_qattr] unfold let va_coerce_operand_to_cmp(o:va_operand{not (TMem? o)}) : va_cmp = o
+[@va_qattr] unfold let va_coerce_operand_to_cmp (o:va_operand{not (TMem? o)}) : va_cmp = o
 [@va_qattr] unfold let va_coerce_opr64_to_cmp (o:va_operand{not (TMem? o)}) : va_cmp = o
 [@va_qattr] unfold let va_op_register (r:reg) : va_register = r
 [@va_qattr] unfold let va_op_reg_oprerand_reg (r:reg) : va_reg_operand = TReg r
@@ -162,12 +190,13 @@ val va_fuel_default : unit -> va_fuel
 [@va_qattr] unfold let va_coerce_operand_to_dst_operand (o:va_operand) : va_dst_operand = o
 [@va_qattr] unfold let va_coerce_dst_operand_to_operand (o:va_dst_operand) : va_operand = o
 [@va_qattr] unfold let va_coerce_dst_opr64_to_opr64 (o:va_dst_operand) : va_operand = o
+
 [@va_qattr]
 unfold let va_opr_code_Mem (o:va_operand) (offset:int) (t:taint) : va_operand =
   match o with
-  | TConst n -> TConst (n + offset)
+  | TConst n -> TMem (MConst (n + offset)) t
   | TReg r -> TMem (MReg r offset) t
-  | _ -> TConst 42
+  | _ -> TMem (MConst 42) t
 
 val va_opr_lemma_Mem (s:va_state) (base:va_operand) (offset:int) (b:M.buffer64) (index:int) (t:taint) : Lemma
   (requires
@@ -176,8 +205,28 @@ val va_opr_lemma_Mem (s:va_state) (base:va_operand) (offset:int) (b:M.buffer64) 
     M.valid_taint_buf64 b s.mem s.memTaint t /\
     eval_operand (t_op_to_op base) s + offset == M.buffer_addr b s.mem + 8 `op_Multiply` index
   )
-  (ensures valid_operand (va_opr_code_Mem base offset t) s /\
-           M.load_mem64 (M.buffer_addr b s.mem + 8 `op_Multiply` index) s.mem == M.buffer_read b index s.mem)
+  (ensures
+    valid_operand (va_opr_code_Mem base offset t) s /\
+    M.load_mem64 (M.buffer_addr b s.mem + 8 `op_Multiply` index) s.mem == M.buffer_read b index s.mem
+  )
+
+[@va_qattr]
+unfold let va_opr_code_Mem128 (o:va_operand) (offset:int) (t:taint) : va_operand128 =
+  match o with
+  | TReg r -> TMem128 (MReg r offset) t
+  | _ -> TMem128 (MConst 42) t
+
+val va_opr_lemma_Mem128 (s:va_state) (base:va_operand) (offset:int) (b:M.buffer128) (index:int) (t:taint) : Lemma
+  (requires
+    TReg? base /\
+    valid_src_addr s.mem b index /\
+    M.valid_taint_buf128 b s.mem s.memTaint t /\
+    eval_operand (t_op_to_op base) s + offset == M.buffer_addr b s.mem + 16 `op_Multiply` index
+  )
+  (ensures
+    valid_operand128 (va_opr_code_Mem128 base offset t) s /\
+    M.load_mem128 (M.buffer_addr b s.mem + 16 `op_Multiply` index) s.mem == M.buffer_read b index s.mem
+  )
 
 val taint_at (memTaint:M.memtaint) (addr:int) : taint
 
@@ -188,7 +237,8 @@ val taint_at (memTaint:M.memtaint) (addr:int) : taint
 [@va_qattr] unfold let va_eval_cmp_uint64   (s:va_state) (r:va_cmp)         : GTot nat64 = eval_operand (t_op_to_op r) s
 [@va_qattr] unfold let va_eval_reg64        (s:va_state) (r:va_register)    : GTot nat64 = eval_reg r s
 [@va_qattr] unfold let va_eval_reg_opr64    (s:va_state) (o:va_operand)     : GTot nat64 = eval_operand (t_op_to_op o) s
-[@va_qattr] unfold let va_eval_xmm          (s:va_state) (x:xmm)            : quad32 = eval_xmm x s
+[@va_qattr] unfold let va_eval_xmm          (s:va_state) (x:xmm)            : GTot quad32 = eval_xmm x s
+[@va_qattr] unfold let va_eval_opr128       (s:va_state) (o:va_operand128)  : GTot quad32 = eval_operand128 (t_op_to_op128 o) s
 
 (* Predicates *)
 [@va_qattr] unfold let va_is_src_opr64 (o:va_operand) (s:va_state) = valid_operand o s
@@ -201,6 +251,7 @@ val taint_at (memTaint:M.memtaint) (addr:int) : taint
 [@va_qattr] unfold let va_is_dst_reg_opr64 (o:va_operand) (s:va_state) = OReg? (t_op_to_op o) /\ not (Rsp? (OReg?.r (t_op_to_op o)))
 [@va_qattr] unfold let va_is_src_xmm (x:xmm) (s:va_state) = True
 [@va_qattr] unfold let va_is_dst_xmm (x:xmm) (s:va_state) = True
+[@va_qattr] unfold let va_is_src_opr128 (o:va_operand128) (s:va_state) = valid_operand128 o s
 
 (* Getters *)
 [@va_qattr] unfold let va_get_ok (s:va_state) : bool = s.ok
