vale/specs/hardware/X64.Bytes_Semantics_s.fst
@@ -632,6 +632,7 @@ let eval_ins (ins:ins) : st unit =
     update_xmm_preserve_flags dst (quad32_xor (eval_xmm dst s) (eval_xmm src s))
 
   |VPxor dst src1 src2 ->
+    check (valid_mov128_op src2);;
     update_xmm_preserve_flags dst (quad32_xor (eval_xmm src1 s) (eval_mov128_op src2 s))
 
   | Pslld dst amt ->
